src/language/reducible.v
@@ -50,16 +50,15 @@ Proof.
   by unfold locs.
 Qed.
 
-Lemma reducible_if maxsize r n t1 t2 σ :
-  reducible maxsize r (tm_if (tm_val (val_nat n)) t1 t2) σ.
+Ltac reduce_easy :=
+  eexists _,_;
+  eapply AltRedGCHead;
+  eauto using gc_id with head_step.
+
+Lemma reducible_if maxsize r b t1 t2 σ :
+  reducible maxsize r (tm_if (tm_val (val_bool b)) t1 t2) σ.
 Proof.
-  destruct (decide (n=0)).
-  { eexists _,_.
-    eapply AltRedGCHead;
-    eauto using gc_id with head_step. }
-  { eexists _,_.
-    eapply AltRedGCHead;
-    eauto using gc_id with head_step. }
+  destruct b; reduce_easy.
 Qed.
 
 Lemma reducible_alloc maxsize r n σ :
@@ -75,14 +74,17 @@ Proof.
   apply is_fresh.
 Qed.
 
-Ltac reduce_easy :=
-  eexists _,_;
-  eapply AltRedGCHead;
-  [ apply gc_id | eauto with head_step].
-
-Lemma reducible_bin_op maxsize r op n m σ :
-  reducible maxsize r (tm_bin_op op (tm_val (val_nat n)) (tm_val (val_nat m))) σ.
-Proof. reduce_easy. Qed.
+Lemma reducible_prim maxsize r p vs σ :
+  is_Some (eval_call_prim p vs) ->
+  reducible maxsize r (tm_call p (tm_val <$> vs)) σ.
+Proof.
+  intros (?,E).
+  destruct p.
+  all: do 2 (try destruct vs as [|?v ?vs]; simpl in E; try congruence).
+  all: try destruct b; try destruct v; simpl in E; try congruence; try destruct v0; simpl in E; try congruence.
+  all: try destruct vs; try congruence.
+  all: injection E; intros; subst; reduce_easy.
+Qed.
 
 Ltac reduce_store_load :=
   intros ? Hn2;
