src/wp_all.v
@@ -1,1 +1,1 @@
-From spacelambda Require Export interp wp_alloc wp_call wp_load wp_bin_op wp_store wpc.
+From spacelambda Require Export interp wp_alloc wp_call wp_load wp_call_prim wp_store wpc.
