src/wp_call_prim.v
@@ -1,0 +1,59 @@
+From iris.proofmode Require Import base proofmode classes.
+From iris.algebra Require Import gmap auth.
+From stdpp Require Import gmap gmultiset.
+
+From spacelambda.spacelang Require Import successors predecessors.
+From spacelambda.language Require Import language.
+
+From spacelambda Require Import more_maps_and_sets.
+From spacelambda Require Import interp.
+
+Section Wp_call_prim.
+
+Context `{!interpGS Σ}.
+
+Lemma locs_result_eval_call_prim p vs x :
+  eval_call_prim p vs = Some x ->
+  locs_val x = ∅.
+Proof.
+  intros E.
+  destruct p.
+  (* XXX tactic, see invert_step *)
+  all: destruct vs as [|?v ?vs]; simpl in E; try congruence.
+  all: try destruct b; try congruence.
+  all: destruct vs as [|?v ?vs]; simpl in E; try congruence.
+  all: destruct v; try congruence.
+  all: try destruct v0; try congruence.
+  all: try destruct vs; try congruence.
+  all: injection E; intros <-; auto_locs; set_solver.
+Qed.
+
+Lemma wp_call_prim b (p:prim) (vs:list val) w :
+  eval_call_prim p vs = Some w ->
+  ⊢ wp b (tm_call p (tm_val <$> vs)) (fun v => ⌜v = w⌝).
+Proof.
+  iIntros (Hw).
+  rewrite wp_unfold /wp_pre. simpl.
+  iIntros.
+  iSplitR.
+  { eauto using reducible_prim. }
+
+  iModIntro.
+  iIntros (? ?) "%Hstep".
+  destruct (invert_step_call_prim _ Hstep) as (Hgc&(?,(?&Hv))). subst.
+
+  iDestruct (interp_gc with "[$]") as "?".
+  { apply (gc_weak Hgc).
+    auto_locs. set_solver. }
+
+  auto_locs. rewrite left_id_L.
+
+  iDestruct (interp_weak with "[$]") as  "?"; last iFrame.
+  { erewrite locs_result_eval_call_prim; eauto. set_solver. }
+  do 2 iModIntro.
+
+  rewrite Hv in Hw. injection Hw. intros ->.
+  iApply wp_val. eauto.
+Qed.
+
+End Wp_call_prim.
